relecture sylvain
avec TODOs pour refactoring #90

mppa_k1c/PostpassSchedulingOracle.ml
@@ -1,4 +1,5 @@
 open Asmvliw
+open Asmblock
 open Printf
 open Camlcoq
 open InstructionScheduler
