mppa_k1c/lib/Asmblockgenproof0.v
@@ -1006,7 +1006,7 @@ Lemma exec_straight_through_singleinst:
 Proof.
   intros. subst. constructor 1. unfold exec_bblock. simpl body. erewrite exec_straight_body; eauto.
   simpl. auto.
-  simpl; auto. unfold nextblock; simpl. Simpl. erewrite exec_straight_pc; eauto.
+  simpl; auto. unfold nextblock, incrPC; simpl. Simpl. erewrite exec_straight_pc; eauto.
 Qed.
 
 (** The following lemmas show that straight-line executions
